capsule-ltl/lean/SecureBootInstance.lean
@@ -21,6 +21,7 @@
 -/
 
 import AuthMonotone
+import ltl_capsule
 
 namespace UefiSecureBoot
 
